progs/verif_queue_ex.v
@@ -1,0 +1,784 @@
+Require Import progs.conclib.
+Require Import progs.verif_conc_queue.
+Require Import progs.queue_ex.
+Require Import SetoidList.
+
+Set Bullet Behavior "Strict Subproofs".
+
+Instance CompSpecs : compspecs. make_compspecs prog. Defined.
+Definition Vprog : varspecs. mk_varspecs prog. Defined.
+
+Definition acquire_spec := DECLARE _acquire acquire_spec.
+Definition release_spec := DECLARE _release release_spec.
+Definition makelock_spec := DECLARE _makelock (makelock_spec _).
+Definition freelock_spec := DECLARE _freelock (freelock_spec _).
+Definition spawn_spec := DECLARE _spawn spawn_spec.
+Definition freelock2_spec := DECLARE _freelock2 (freelock2_spec _).
+Definition release2_spec := DECLARE _release2 release2_spec.
+Definition makecond_spec := DECLARE _makecond (makecond_spec _).
+Definition freecond_spec := DECLARE _freecond (freecond_spec _).
+Definition wait_spec := DECLARE _waitcond (wait2_spec _).
+Definition signal_spec := DECLARE _signalcond (signal_spec _).
+
+Definition f_lock_pred lsh gsh tsh gsh1 gsh2 p' p lock tid t locksp lockt resultsp :=
+  selflock (EX v1 : val, EX v2 : val, EX v3 : val, EX h : hist, data_at gsh (tptr tqueue_t) p p' *
+            lqueue lsh tint p lock gsh1 gsh2 h * data_at Tsh tint (vint t) tid *
+            field_at Ews (tarray (tptr tlock) 3) [ArraySubsc t] lockt locksp *
+            field_at Ews (tarray (tarray tint 3) 3) [ArraySubsc t] [v1; v2; v3] resultsp *
+            ghost gsh1 (lsh, [QRem v1; QRem v2; QRem v3]) p])) tsh lockt.
+
+Definition f_spec :=
+ DECLARE _f
+  WITH tid : val, x : share * share * share * share * share * val * val * val * Z * val * val * val
+  PRE [ _arg OF (tptr tvoid) ]
+   let '(lsh, gsh, tsh, gsh1, gsh2, p', p, lock, t, locksp, lockt, resultsp, h) := x in
+   PROP ()
+   LOCAL (temp _arg tid; gvar _q0 p'; gvar _thread_locks locksp; gvar _results resultsp)
+   SEP (!!(readable_share lsh /\ readable_share gsh /\ readable_share tsh /\ sepalg.join gsh1 gsh2 Tsh) && emp;
+        data_at gsh (tptr tqueue_t) p p'; lqueue lsh tint p lock gsh1 gsh2 [];
+        data_at Tsh tint (vint t) tid;
+        field_at Ews (tarray (tptr tlock) 3) [ArraySubsc t] lockt locksp;
+        field_at_ Ews (tarray (tarray tint 3) 3) [ArraySubsc t] resultsp;
+        lock_inv tsh lockt (f_lock_pred lsh gsh tsh gsh1 gsh2 p' p lock tid t locksp lockt resultsp))
+  POST [ tptr tvoid ] PROP () LOCAL () SEP (emp).
+
+Definition main_spec :=
+ DECLARE _main
+  WITH u : unit
+  PRE  [] main_pre prog [] u
+  POST [ tint ] main_post prog [] u.
+
+Definition Gprog : funspecs := augment_funspecs prog [acquire_spec; release_spec; release2_spec; makelock_spec;
+  freelock_spec; freelock2_spec; spawn_spec; makecond_spec; freecond_spec; wait_spec; signal_spec;
+  malloc_spec; free_spec;
+  q_new_spec; q_del_spec; q_add_spec; q_remove_spec; f_spec; main_spec].
+
+Lemma f_inv_precise : forall lsh gsh tsh p' p lock lockt ghosts gsh2 (Hlsh : readable_share lsh)
+  (Hgsh : readable_share gsh),
+  precise (Interp (f_lock_pred lsh gsh tsh p' p lock lockt ghosts gsh2)).
+Proof.
+  intros; simpl.
+  apply selflock_precise; repeat apply precise_sepcon; auto.
+  apply lock_precise; auto.
+Qed.
+
+Lemma f_inv_positive : forall lsh gsh tsh p' p lock lockt ghosts gsh2,
+  positive_mpred (Interp (f_lock_pred lsh gsh tsh p' p lock lockt ghosts gsh2)).
+Proof.
+  intros; apply selflock_positive.
+  simpl; apply positive_sepcon2, positive_sepcon2, positive_sepcon1, lock_inv_positive.
+Qed.
+
+Lemma body_f : semax_body Vprog Gprog f_f f_spec.
+Proof.
+  start_function.
+  rewrite (lock_inv_isptr _ lockt); Intros.
+  unfold lqueue; rewrite field_at_isptr; Intros.
+  forward.
+  match goal with |-semax _ ?P _ _ => forward_for_simple_bound 3 (EX i : Z, P) end.
+  { entailer. }
+  { forward_call tt.
+    Intro x; destruct x as ((req, d), t).
+    forward_call (lsh, p, lock, req, d, t, ghosts, gsh2).
+    { unfold lqueue; cancel. }
+    unfold lqueue; entailer!. }
+  forward_call (lockt, tsh, f_lock_pred lsh gsh tsh p' p lock lockt ghosts gsh2).
+  { simpl.
+    rewrite selflock_eq at 2; cancel.
+    subst Frame; instantiate (1 := []); normalize; apply lock_inv_later. }
+  { split; auto; repeat split; [apply f_inv_precise | apply f_inv_positive | apply selflock_rec]; auto. }
+  forward.
+Qed.
+
+Lemma lock_struct : forall p, data_at_ Tsh (Tstruct _lock_t noattr) p |-- data_at_ Tsh tlock p.
+Proof.
+  intros.
+  unfold data_at_, field_at_; unfold_field_at 1%nat; simpl.
+  unfold field_at; simpl.
+  rewrite field_compatible_cons; simpl; entailer.
+Qed.
+
+Lemma lock_struct_array : forall z p, data_at_ Tsh (tarray (Tstruct _lock_t noattr) z) p |--
+  data_at_ Tsh (tarray tlock z) p.
+Proof.
+  intros.
+  unfold data_at_, field_at_, field_at; simpl; entailer.
+  unfold default_val, at_offset; simpl.
+  do 2 rewrite data_at_rec_eq; simpl.
+  unfold array_pred, aggregate_pred.array_pred, unfold_reptype; simpl; entailer.
+  rewrite Z.sub_0_r; clear.
+  forget (Z.to_nat z) as l; forget 0 as lo; revert lo; induction l; intros; simpl; auto.
+  apply sepcon_derives.
+  - unfold at_offset; rewrite data_at_rec_eq; simpl.
+    unfold struct_pred, aggregate_pred.struct_pred, at_offset, withspacer; simpl; entailer.
+  - eapply derives_trans; [apply aggregate_pred.rangespec_ext_derives |
+      eapply derives_trans; [apply IHl | apply aggregate_pred.rangespec_ext_derives]]; simpl; intros;
+      rewrite Znth_pos_cons; try omega; replace (i - lo - 1) with (i - Z.succ lo) by omega; auto.
+Qed.
+
+(*Lemma main_loop1 : forall {Espec : OracleKind} (q0 lvar0 : val) gsh1 gsh2 (Hgsh1 : readable_share gsh1) (Hgsh2 : readable_share gsh2)
+  (Hgsh : sepalg.join gsh1 gsh2 Ews) g1 g2 g3 (ghosts := [g1; g2; g3]) p lock lshs1 (Hlenl1 : Zlength lshs1 = 3)
+  (Hlshs1 : forall i : Z, 0 <= i < 3 -> let '(a, b) := Znth i lshs1 (Tsh, Tsh) in
+          readable_share a /\ readable_share b /\ sepalg.join a b (fst (Znth (i + 1) lshs1 (Tsh, Tsh))))
+  gshs1 (Hglen1 : Zlength gshs1 = 3)
+  (Hgshs1 : forall i : Z, 0 <= i < 3 -> let '(a, b) := Znth i gshs1 (Ews, Ews) in
+          readable_share a /\ readable_share b /\ sepalg.join a b (fst (Znth (i + 1) gshs1 (Ews, Ews))))
+  sh1 sh2 (Hsh1 : readable_share sh1) (Hsh2 : readable_share sh2) (Hsh : sepalg.join sh1 sh2 Tsh)
+  (f_lock := fun x : Z * val =>
+          Lock_inv sh1 (snd x)
+            (f_lock_pred (snd (Znth (2 - fst x) lshs1 (Tsh, Tsh))) (snd (Znth (2 - fst x) gshs1 (Ews, Ews))) sh2
+               q0 p lock (snd x) ghosts gsh2)) i (Hi : 0 <= i < 3),
+ semax (initialized_list [_i; _t'1] (func_tycontext f_main Vprog Gprog))
+  (PROP ( )
+   LOCAL (temp _i (vint i); temp _t'1 p; lvar _thread_locks (tarray (tptr (Tstruct _lock_t noattr)) 6) lvar0;
+   gvar _q0 q0)
+   SEP (ghost_factory; data_at (fst (Znth (3 - i) gshs1 (Ews, Ews))) (tptr tqueue_t) p q0;
+   lqueue (fst (Znth (3 - i) lshs1 (Tsh, Tsh))) gsh2 p ghosts lock; ghost gsh1 tint (vint (-1)) g1;
+   ghost gsh1 tint (vint (-1)) g2; ghost gsh1 tint (vint (-1)) g3;
+   EX flocks : list val,
+   !! (Zlength flocks = i) &&
+   (data_at Tsh (tarray (tptr (Tstruct _lock_t noattr)) 6) (flocks ++ repeat Vundef (Z.to_nat (6 - i))) lvar0 *
+    fold_right sepcon emp (map Interp (map f_lock (combine (upto (Z.to_nat i)) flocks))))))
+  (Ssequence
+     (Ssequence
+        (Scall (Some _t'2) (Evar _malloc (Tfunction (Ctypes.Tcons tuint Ctypes.Tnil) (tptr tvoid) cc_default))
+           [Esizeof (Tstruct _lock_t noattr) tuint])
+        (Sset _l (Ecast (Etempvar _t'2 (tptr tvoid)) (tptr (Tstruct _lock_t noattr)))))
+     (Ssequence
+        (Sassign
+           (Ederef
+              (Ebinop Oadd (Evar _thread_locks (tarray (tptr (Tstruct _lock_t noattr)) 6)) 
+                 (Etempvar _i tint) (tptr (tptr (Tstruct _lock_t noattr)))) (tptr (Tstruct _lock_t noattr)))
+           (Etempvar _l (tptr (Tstruct _lock_t noattr))))
+        (Ssequence
+           (Scall None (Evar _makelock (Tfunction (Ctypes.Tcons (tptr tvoid) Ctypes.Tnil) tvoid cc_default))
+              [Ecast (Etempvar _l (tptr (Tstruct _lock_t noattr))) (tptr tvoid)])
+           (Scall None
+              (Evar _spawn
+                 (Tfunction
+                    (Ctypes.Tcons
+                       (tptr (Tfunction (Ctypes.Tcons (tptr tvoid) Ctypes.Tnil) (tptr tvoid) cc_default))
+                       (Ctypes.Tcons (tptr tvoid) Ctypes.Tnil)) tvoid cc_default))
+              [Ecast
+                 (Eaddrof (Evar _f (Tfunction (Ctypes.Tcons (tptr tvoid) Ctypes.Tnil) (tptr tvoid) cc_default))
+                    (tptr (Tfunction (Ctypes.Tcons (tptr tvoid) Ctypes.Tnil) (tptr tvoid) cc_default)))
+                 (tptr tvoid); Ecast (Etempvar _l (tptr (Tstruct _lock_t noattr))) (tptr tvoid)]))))
+  (normal_ret_assert
+     (PROP (0 <= i + 1 <= 3)
+      LOCAL (temp _i (vint i); temp _t'1 p; lvar _thread_locks (tarray (tptr (Tstruct _lock_t noattr)) 6) lvar0;
+      gvar _q0 q0)
+      SEP (ghost_factory; data_at (fst (Znth (3 - (i + 1)) gshs1 (Ews, Ews))) (tptr tqueue_t) p q0;
+      lqueue (fst (Znth (3 - (i + 1)) lshs1 (Tsh, Tsh))) gsh2 p ghosts lock; ghost gsh1 tint (vint (-1)) g1;
+      ghost gsh1 tint (vint (-1)) g2; ghost gsh1 tint (vint (-1)) g3;
+      EX flocks : list val,
+      !! (Zlength flocks = i + 1) &&
+      (data_at Tsh (tarray (tptr (Tstruct _lock_t noattr)) 6) (flocks ++ repeat Vundef (Z.to_nat (6 - (i + 1))))
+         lvar0 * fold_right sepcon emp (map Interp (map f_lock (combine (upto (Z.to_nat (i + 1))) flocks))))))).
+Proof.
+  intros.
+  forward_call (sizeof tlock).
+  { simpl fold_right; cancel. }
+  { simpl; computable. }
+  Intros l flocks.
+  forward.
+  rewrite upd_Znth_app2; [|repeat rewrite Zlength_correct in *; abstract omega].
+  replace (i - Zlength flocks) with 0 by abstract omega; rewrite upd_Znth0, sublist_repeat;
+    try rewrite Zlength_repeat, Z2Nat.id; try abstract omega.
+  assert (isptr l) by (destruct l; try contradiction; simpl; auto).
+  forward_call (l, Tsh, f_lock_pred (snd (Znth (2 - i) lshs1 (Tsh, Tsh)))
+    (snd (Znth (2 - i) gshs1 (Ews, Ews))) sh2 q0 p lock l ghosts gsh2).
+  { rewrite !sem_cast_neutral_ptr; auto; apply prop_right; auto. }
+  { repeat rewrite sepcon_assoc; apply sepcon_derives; [|cancel].
+    rewrite memory_block_data_at_;
+      [simpl; cancel | apply malloc_field_compatible; auto; simpl; try computable].
+    exists 2; auto. }
+  get_global_function'' _f; Intros.
+  apply extract_exists_pre; intros f_.
+  match goal with |-context[func_ptr' ?P] => set (spec := P) end.
+  forward_call (f_, l, existT (fun ty => ty * (ty -> val -> Pred))%type
+    (share * share * share * val * val * val * list val * share)%type
+    ((snd (Znth (2 - i) lshs1 (Tsh, Tsh)), snd (Znth (2 - i) gshs1 (Ews, Ews)),
+     sh2, q0, p, lock, ghosts, gsh2),
+   fun (x : (share * share * share * val * val * val * list val * share)) (lockt : val) =>
+   let '(lsh, gsh, tsh, p', p, lock, ghosts, gsh2) := x in
+   Pred_list [Pred_prop (readable_share lsh /\ readable_share gsh /\ readable_share tsh);
+     Data_at _ gsh (tptr tqueue_t) p p'; 
+     Field_at _ lsh tqueue_t [StructField _lock] lock p;
+     Lock_inv lsh lock (lock_pred gsh2 p ghosts);
+     Lock_inv tsh lockt (f_lock_pred lsh gsh tsh p' p lock lockt ghosts gsh2)])).
+  { apply prop_right; destruct l; try contradiction; auto. }
+  { Exists _arg (fun x : share * share * share * val * val * val * list val * share =>
+      let '(_, _, _, p', _, _, _, _) := x in [(_q0, p')]).
+    repeat rewrite sepcon_assoc; apply sepcon_derives.
+    { apply derives_refl'.
+      subst spec; f_equal; f_equal.
+      extensionality.
+      destruct x as (?, (((((((?, ?), ?), ?), ?), ?), ?), ?)); simpl.
+      f_equal; f_equal.
+      unfold SEPx, lqueue; simpl; normalize. }
+    subst Frame; instantiate (1 := [ghost_factory;
+      data_at (fst (Znth (2 - i) gshs1 (Ews, Ews))) (tptr tqueue_t) p q0;
+      lqueue (fst (Znth (2 - i) lshs1 (Tsh, Tsh))) gsh2 p ghosts lock;
+      ghost gsh1 tint (vint (-1)) g1; ghost gsh1 tint (vint (-1)) g2; ghost gsh1 tint (vint (-1)) g3;
+      data_at Tsh (tarray (tptr (Tstruct _lock_t noattr)) 6) ((flocks ++ [l]) ++ repeat Vundef (Z.to_nat (6 - (i + 1)))) lvar0;
+      fold_right sepcon emp (map Interp (map f_lock (combine (upto (Z.to_nat (i + 1))) (flocks ++ [l]))))]).
+    rewrite <- (lock_inv_share_join sh1 sh2 Tsh); auto.
+    specialize (Hgshs1 (2 - i)); exploit Hgshs1; [abstract omega|].
+    destruct (Znth (2 - i) gshs1 (Ews, Ews)) eqn: Hg1.
+    replace (2 - i + 1) with (3 - i) by abstract omega.
+    intros (? & ? & Hglsh); rewrite <- (data_at_share_join _ _ _ _ _ _ Hglsh); auto.
+    specialize (Hlshs1 (2 - i)); exploit Hlshs1; [abstract omega|].
+    destruct (Znth (2 - i) lshs1 (Tsh, Tsh)) eqn: Hl1.
+    replace (2 - i + 1) with (3 - i) by abstract omega.
+    intros (? & ? & Hllsh); rewrite <- (lqueue_share_join s s0 (fst (Znth (3 - i) lshs1 (Tsh, Tsh)))); auto.
+    unfold lqueue; simpl; rewrite Z.sub_add_distr, <- app_assoc; simpl.
+    repeat rewrite Hg1; repeat rewrite Hl1; simpl.
+    repeat rewrite sepcon_andp_prop'; apply andp_right; [apply prop_right; auto | cancel].
+    rewrite Z2Nat.inj_add, upto_app, combine_app; try abstract omega.
+    simpl; repeat rewrite map_app; simpl.
+    rewrite Z2Nat.id, Z.add_0_r, Hg1, Hl1; simpl; [|abstract omega].
+    rewrite sem_cast_neutral_ptr; auto.
+    rewrite sepcon_app; simpl; unfold fold_right at 2; cancel.
+    { rewrite upto_length; rewrite Zlength_correct in *; Omega0. } }
+  entailer!.
+  replace (3 - (Zlength flocks + 1)) with (2 - Zlength flocks) by abstract omega.
+  Exists (flocks ++ [l]); rewrite Zlength_app, Zlength_cons, Zlength_nil; entailer!.
+Qed.
+
+Lemma main_loop2 : forall {Espec : OracleKind} (q0 lvar0 : val) gsh1 gsh2 (Hgsh1 : readable_share gsh1) (Hgsh2 : readable_share gsh2)
+  (Hgsh : sepalg.join gsh1 gsh2 Ews) g1 g2 g3 (ghosts := [g1; g2; g3]) p lock lshs1 (Hlenl1 : Zlength lshs1 = 3)
+  (Hlshs1 : forall i : Z, 0 <= i < 3 -> let '(a, b) := Znth i lshs1 (Tsh, Tsh) in
+          readable_share a /\ readable_share b /\ sepalg.join a b (fst (Znth (i + 1) lshs1 (Tsh, Tsh))))
+  gshs1 (Hglen1 : Zlength gshs1 = 3)
+  (Hgshs1 : forall i : Z, 0 <= i < 3 -> let '(a, b) := Znth i gshs1 (Ews, Ews) in
+          readable_share a /\ readable_share b /\ sepalg.join a b (fst (Znth (i + 1) gshs1 (Ews, Ews))))
+  sh1 sh2 (Hsh1 : readable_share sh1) (Hsh2 : readable_share sh2) (Hsh : sepalg.join sh1 sh2 Tsh)
+  (f_lock := fun x : Z * val =>
+          Lock_inv sh1 (snd x)
+            (f_lock_pred (snd (Znth (2 - fst x) lshs1 (Tsh, Tsh))) (snd (Znth (2 - fst x) gshs1 (Ews, Ews))) sh2
+               q0 p lock (snd x) ghosts gsh2)) flocks (Hflocks : Zlength flocks = 3)
+  (lsh' := fst (Znth 0 lshs1 (Tsh, Tsh))) (gsh' := fst (Znth 0 gshs1 (Ews, Ews)))
+  lshs2 (Hlenl2 : Zlength lshs2 = 3)
+  (Hlshs2 : forall i : Z, 0 <= i < 3 -> let '(a, b) := Znth i lshs2 (lsh', lsh') in
+          readable_share a /\ readable_share b /\ sepalg.join a b (fst (Znth (i + 1) lshs2 (lsh', lsh'))))
+  gshs2 (Hglen2 : Zlength gshs2 = 3)
+  (Hgshs2 : forall i : Z, 0 <= i < 3 -> let '(a, b) := Znth i gshs2 (gsh', gsh') in
+          readable_share a /\ readable_share b /\ sepalg.join a b (fst (Znth (i + 1) gshs2 (gsh', gsh'))))
+  (g_lock := fun x : Z * val => Lock_inv sh1 (snd x)
+            (g_lock_pred (snd (Znth (2 - fst x) lshs2 (lsh', lsh'))) (snd (Znth (2 - fst x) gshs2 (gsh', gsh')))
+               sh2 q0 p lock (snd x) ghosts gsh1 gsh2 (Znth (fst x) ghosts Vundef))) i (Hi : 0 <= i < 3),
+semax (initialized_list [_i; _i__1; _t'1] (func_tycontext f_main Vprog Gprog))
+  (PROP (Zlength flocks = 3)
+   LOCAL (temp _i__1 (vint i); temp _t'1 p; lvar _thread_locks (tarray (tptr (Tstruct _lock_t noattr)) 6) lvar0;
+   gvar _q0 q0)
+   SEP (ghost_factory; data_at (fst (Znth (3 - i) gshs2 (gsh', gsh'))) (tptr tqueue_t) p q0;
+   lqueue (fst (Znth (3 - i) lshs2 (lsh', lsh'))) gsh2 p ghosts lock;
+   fold_right sepcon emp (skipn (Z.to_nat i) (map (ghost gsh1 tint (vint (-1))) ghosts));
+   fold_right sepcon emp (map Interp (map f_lock (combine (upto 3) flocks)));
+   EX glocks : list val,
+   !! (Zlength glocks = i) &&
+   (data_at Tsh (tarray (tptr (Tstruct _lock_t noattr)) 6) (flocks ++ glocks ++ repeat Vundef (Z.to_nat (3 - i)))
+      lvar0 * fold_right sepcon emp (map Interp (map g_lock (combine (upto (Z.to_nat i)) glocks))))))
+  (Ssequence
+     (Ssequence
+        (Scall (Some _t'3) (Evar _malloc (Tfunction (Ctypes.Tcons tuint Ctypes.Tnil) (tptr tvoid) cc_default))
+           [Esizeof (Tstruct _lock_t noattr) tuint])
+        (Sset _l__1 (Ecast (Etempvar _t'3 (tptr tvoid)) (tptr (Tstruct _lock_t noattr)))))
+     (Ssequence
+        (Sassign
+           (Ederef
+              (Ebinop Oadd (Evar _thread_locks (tarray (tptr (Tstruct _lock_t noattr)) 6))
+                 (Ebinop Oadd (Etempvar _i__1 tint) (Econst_int (Int.repr 3) tint) tint)
+                 (tptr (tptr (Tstruct _lock_t noattr)))) (tptr (Tstruct _lock_t noattr)))
+           (Etempvar _l__1 (tptr (Tstruct _lock_t noattr))))
+        (Ssequence
+           (Scall None (Evar _makelock (Tfunction (Ctypes.Tcons (tptr tvoid) Ctypes.Tnil) tvoid cc_default))
+              [Ecast (Etempvar _l__1 (tptr (Tstruct _lock_t noattr))) (tptr tvoid)])
+           (Scall None
+              (Evar _spawn
+                 (Tfunction
+                    (Ctypes.Tcons
+                       (tptr (Tfunction (Ctypes.Tcons (tptr tvoid) Ctypes.Tnil) (tptr tvoid) cc_default))
+                       (Ctypes.Tcons (tptr tvoid) Ctypes.Tnil)) tvoid cc_default))
+              [Ecast
+                 (Eaddrof (Evar _g (Tfunction (Ctypes.Tcons (tptr tvoid) Ctypes.Tnil) (tptr tvoid) cc_default))
+                    (tptr (Tfunction (Ctypes.Tcons (tptr tvoid) Ctypes.Tnil) (tptr tvoid) cc_default)))
+                 (tptr tvoid); Ecast (Etempvar _l__1 (tptr (Tstruct _lock_t noattr))) (tptr tvoid)]))))
+  (normal_ret_assert
+     (PROP (0 <= i + 1 <= 3; Zlength flocks = 3)
+      LOCAL (temp _i__1 (vint i); temp _t'1 p;
+      lvar _thread_locks (tarray (tptr (Tstruct _lock_t noattr)) 6) lvar0; gvar _q0 q0)
+      SEP (ghost_factory; data_at (fst (Znth (3 - (i + 1)) gshs2 (gsh', gsh'))) (tptr tqueue_t) p q0;
+      lqueue (fst (Znth (3 - (i + 1)) lshs2 (lsh', lsh'))) gsh2 p ghosts lock;
+      fold_right sepcon emp (skipn (Z.to_nat (i + 1)) (map (ghost gsh1 tint (vint (-1))) ghosts));
+      fold_right sepcon emp (map Interp (map f_lock (combine (upto 3) flocks)));
+      EX glocks : list val,
+      !! (Zlength glocks = i + 1) &&
+      (data_at Tsh (tarray (tptr (Tstruct _lock_t noattr)) 6)
+         (flocks ++ glocks ++ repeat Vundef (Z.to_nat (3 - (i + 1)))) lvar0 *
+       fold_right sepcon emp (map Interp (map g_lock (combine (upto (Z.to_nat (i + 1))) glocks))))))).
+Proof.
+  intros.
+  forward_call (sizeof tlock).
+    { simpl fold_right; cancel. }
+    { simpl; computable. }
+    Intros l glocks.
+    forward.
+    rewrite app_assoc, upd_Znth_app2; [|rewrite Zlength_app, Zlength_repeat; abstract omega].
+    rewrite Zlength_app; replace (i + 3 - (Zlength flocks + Zlength glocks)) with 0 by abstract omega.
+    rewrite upd_Znth0, sublist_repeat; try rewrite Zlength_repeat, Z2Nat.id; try abstract omega.
+    assert (isptr l) by (destruct l; try contradiction; simpl; auto).
+    forward_call (l, Tsh, g_lock_pred (snd (Znth (2 - i) lshs2 (lsh', lsh')))
+      (snd (Znth (2 - i) gshs2 (gsh', gsh'))) sh2 q0 p lock l ghosts gsh1 gsh2 (Znth i ghosts Vundef)).
+    { repeat rewrite sem_cast_neutral_ptr; auto; apply prop_right; auto. }
+    { repeat rewrite sepcon_assoc; apply sepcon_derives; [|cancel].
+      rewrite memory_block_data_at_; [simpl; cancel | apply malloc_field_compatible; auto; simpl; try computable].
+      exists 2; auto. }
+    get_global_function'' _g; Intros.
+    apply extract_exists_pre; intros g_.
+    match goal with |-context[func_ptr' ?P] => set (spec := P) end.
+    forward_call (g_, l, existT (fun ty => ty * (ty -> val -> Pred))%type
+      (share * share * share * Z * val * val * val * list val * nat * val * share * share)%type
+      ((snd (Znth (2 - i) lshs2 (lsh', lsh')), snd (Znth (2 - i) gshs2 (gsh', gsh')),
+       sh2, -1, q0, p, lock, ghosts, Z.to_nat i, Znth i ghosts Vundef, gsh1, gsh2),
+     fun (x : (share * share * share * Z * val * val * val * list val * nat * val * share * share)) (lockt : val) =>
+     let '(lsh, gsh, tsh, t, p', p, lock, ghosts, i, g, gsh1, gsh2) := x in
+     Pred_list [Pred_prop (readable_share lsh /\ readable_share gsh /\ readable_share tsh /\
+         Int.min_signed <= t <= Int.max_signed /\ sepalg.join gsh1 gsh2 Ews /\ nth_error ghosts i = Some g);
+       Data_at _ gsh (tptr tqueue_t) p p'; 
+       Field_at _ lsh tqueue_t [StructField _lock] lock p;
+       Lock_inv lsh lock (lock_pred gsh2 p ghosts);
+       Lock_inv tsh lockt (g_lock_pred lsh gsh tsh p' p lock lockt ghosts gsh1 gsh2 g);
+       Ghost gsh1 tint (vint t) g])).
+    { apply prop_right; destruct l; try contradiction; auto. }
+    { unfold fold_right at 1.
+      Exists _arg (fun x : share * share * share * Z * val * val * val * list val * nat * val * share * share =>
+        let '(_, _, _, _, p', _, _, _, _, _, _, _) := x in [(_q0, p')]).
+      repeat rewrite sepcon_assoc; apply sepcon_derives.
+      { apply derives_refl'.
+        subst spec; f_equal; f_equal.
+        extensionality.
+        destruct x as (?, (((((((((((?, ?), ?), ?), ?), ?), ?), ?), ?), ?), ?), ?)); simpl.
+        rewrite interp_ghost; f_equal; f_equal.
+        unfold SEPx, lqueue; simpl; normalize. }
+      subst Frame; instantiate (1 := [ghost_factory;
+        data_at (fst (Znth (2 - i) gshs2 (gsh', gsh'))) (tptr tqueue_t) p q0;
+        lqueue (fst (Znth (2 - i) lshs2 (lsh', lsh'))) gsh2 p ghosts lock;
+        fold_right sepcon emp (skipn (Z.to_nat (i + 1)) (map (ghost gsh1 tint (vint (-1))) ghosts));
+        fold_right sepcon emp (map Interp (map f_lock (combine (upto 3) flocks)));
+        data_at Tsh (tarray (tptr (Tstruct _lock_t noattr)) 6) (flocks ++ (glocks ++ [l]) ++ repeat Vundef (Z.to_nat (3 - (i + 1)))) lvar0;
+        fold_right sepcon emp (map Interp (map g_lock (combine (upto (Z.to_nat (i + 1))) (glocks ++ [l]))))]).
+      rewrite <- (lock_inv_share_join sh1 sh2 Tsh); auto.
+      exploit (Hgshs2 (2 - i)); [abstract omega|].
+      fold gsh'; destruct (Znth (2 - i) gshs2 (gsh', gsh')) eqn: Hg1.
+      replace (2 - i + 1) with (3 - i) by abstract omega.
+      intros (? & ? & Hglsh); rewrite <- (data_at_share_join _ _ _ _ _ _ Hglsh).
+      exploit (Hlshs2 (2 - i)); [abstract omega|].
+      fold lsh'; destruct (Znth (2 - i) lshs2 (lsh', lsh')) eqn: Hl1.
+      replace (2 - i + 1) with (3 - i) by abstract omega.
+      intros (? & ? & Hllsh); rewrite <- (lqueue_share_join s s0 (fst (Znth (3 - i) lshs2 (lsh', lsh'))));
+        auto.
+      unfold lqueue; simpl; rewrite Z.sub_add_distr, <- app_assoc; simpl.
+      repeat rewrite Hg1; repeat rewrite Hl1; rewrite <- app_assoc; simpl.
+      repeat rewrite sepcon_andp_prop'; apply andp_right; [apply prop_right | unfold fold_right; cancel].
+      { split; [|split; [|split; [|split; [|split]]]]; auto; try computable.
+        unfold Znth; destruct (zlt i 0); [abstract omega|].
+        subst ghosts; erewrite nth_error_nth; simpl; eauto; Omega0. }
+      rewrite Z2Nat.inj_add, upto_app, combine_app; try abstract omega.
+      simpl; repeat rewrite map_app; simpl.
+      rewrite Z.add_0_r, Z2Nat.id; simpl; [|abstract omega].
+      rewrite sepcon_app; simpl; unfold fold_right; cancel.
+      erewrite <- (firstn_skipn 1 (skipn (Z.to_nat i) _)), skipn_skipn,
+        <- firstn_1_skipn with (d := ghost gsh1 tint (vint (-1)) Vundef), sepcon_app; [|Omega0].
+      rewrite nth_Znth, Z2Nat.id; [simpl | abstract omega].
+      rewrite Hg1, Hl1, sem_cast_neutral_ptr; auto.
+      erewrite interp_ghost, <- Znth_map' with (f := ghost _ _ _); subst ghosts; simpl;
+        unfold fold_right; cancel.
+      { subst; rewrite Zlength_correct, Nat2Z.id, upto_length; auto. } }
+    go_lower; Exists (glocks ++ [l]); entailer!.
+    - rewrite Zlength_app, Zlength_cons, Zlength_nil; auto.
+    - replace (3 - (Zlength glocks + 1)) with (2 - Zlength glocks) by abstract omega; apply derives_refl.
+Qed.
+
+Opaque upto.
+
+Lemma main_loop3 : forall {Espec : OracleKind} (q0 lvar0 : val) gsh1 gsh2 (Hgsh1 : readable_share gsh1) (Hgsh2 : readable_share gsh2)
+  (Hgsh : sepalg.join gsh1 gsh2 Ews) g1 g2 g3 (ghosts := [g1; g2; g3]) p lock lshs1 (Hlenl1 : Zlength lshs1 = 3)
+  (Hlshs1 : forall i : Z, 0 <= i < 3 -> let '(a, b) := Znth i lshs1 (Tsh, Tsh) in
+          readable_share a /\ readable_share b /\ sepalg.join a b (fst (Znth (i + 1) lshs1 (Tsh, Tsh))))
+  gshs1 (Hglen1 : Zlength gshs1 = 3)
+  (Hgshs1 : forall i : Z, 0 <= i < 3 -> let '(a, b) := Znth i gshs1 (Ews, Ews) in
+          readable_share a /\ readable_share b /\ sepalg.join a b (fst (Znth (i + 1) gshs1 (Ews, Ews))))
+  sh1 sh2 (Hsh1 : readable_share sh1) (Hsh2 : readable_share sh2) (Hsh : sepalg.join sh1 sh2 Tsh)
+  (f_lock := fun x : Z * val =>
+          Lock_inv sh1 (snd x)
+            (f_lock_pred (snd (Znth (2 - fst x) lshs1 (Tsh, Tsh))) (snd (Znth (2 - fst x) gshs1 (Ews, Ews))) sh2
+               q0 p lock (snd x) ghosts gsh2)) flocks (Hflocks : Zlength flocks = 3)
+  (lsh' := fst (Znth 0 lshs1 (Tsh, Tsh))) (gsh' := fst (Znth 0 gshs1 (Ews, Ews)))
+  lshs2 (Hlenl2 : Zlength lshs2 = 3)
+  (Hlshs2 : forall i : Z, 0 <= i < 3 -> let '(a, b) := Znth i lshs2 (lsh', lsh') in
+          readable_share a /\ readable_share b /\ sepalg.join a b (fst (Znth (i + 1) lshs2 (lsh', lsh'))))
+  gshs2 (Hglen2 : Zlength gshs2 = 3)
+  (Hgshs2 : forall i : Z, 0 <= i < 3 -> let '(a, b) := Znth i gshs2 (gsh', gsh') in
+          readable_share a /\ readable_share b /\ sepalg.join a b (fst (Znth (i + 1) gshs2 (gsh', gsh'))))
+  (g_lock := fun x : Z * val => Lock_inv sh1 (snd x)
+            (g_lock_pred (snd (Znth (2 - fst x) lshs2 (lsh', lsh'))) (snd (Znth (2 - fst x) gshs2 (gsh', gsh')))
+               sh2 q0 p lock (snd x) ghosts gsh1 gsh2 (Znth (fst x) ghosts Vundef)))
+  glocks (Hglocks : Zlength glocks = 3) i (Hi : 0 <= i < 6),
+semax (initialized_list [_i; _i__1; _i__2; _t'1] (func_tycontext f_main Vprog Gprog))
+  (PROP (Forall isptr flocks; Forall isptr glocks)
+   LOCAL (temp _i__2 (vint i); temp _t'1 p; lvar _thread_locks (tarray (tptr (Tstruct _lock_t noattr)) 6) lvar0;
+   gvar _q0 q0)
+   SEP (ghost_factory; data_at (fst (Znth 0 gshs2 (gsh', gsh'))) (tptr tqueue_t) p q0;
+   fold_right sepcon emp
+     (firstn (Z.to_nat i)
+        (map (fun sh : Share.t => data_at sh (tptr tqueue_t) p q0) (map snd (rev gshs1 ++ rev gshs2))));
+   lqueue (fst (Znth 0 lshs2 (lsh', lsh'))) gsh2 p ghosts lock;
+   fold_right sepcon emp
+     (firstn (Z.to_nat i)
+        (map (fun sh : Share.t => lqueue sh gsh2 p ghosts lock) (map snd (rev lshs1 ++ rev lshs2))));
+   EX ns : list Z,
+   !! (Zlength ns = Zlength ghosts) &&
+   fold_right sepcon emp
+     (firstn (Z.to_nat i - 3) (map (fun x : Z * val => ghost gsh1 tint (vint (fst x)) (snd x)) (combine ns ghosts)));
+   fold_right sepcon emp (skipn (Z.to_nat i) (map Interp (map f_lock (combine (upto 3) flocks))));
+   fold_right sepcon emp (skipn (Z.to_nat i - 3) (map Interp (map g_lock (combine (upto 3) glocks))));
+   data_at Tsh (tarray (tptr (Tstruct _lock_t noattr)) 6) (flocks ++ glocks) lvar0))
+  (Ssequence
+     (Sset _l__2
+        (Ederef
+           (Ebinop Oadd (Evar _thread_locks (tarray (tptr (Tstruct _lock_t noattr)) 6)) 
+              (Etempvar _i__2 tint) (tptr (tptr (Tstruct _lock_t noattr)))) (tptr (Tstruct _lock_t noattr))))
+     (Ssequence
+        (Scall None (Evar _acquire (Tfunction (Ctypes.Tcons (tptr tvoid) Ctypes.Tnil) tvoid cc_default))
+           [Ecast (Etempvar _l__2 (tptr (Tstruct _lock_t noattr))) (tptr tvoid)])
+        (Ssequence
+           (Scall None (Evar _freelock2 (Tfunction (Ctypes.Tcons (tptr tvoid) Ctypes.Tnil) tvoid cc_default))
+              [Ecast (Etempvar _l__2 (tptr (Tstruct _lock_t noattr))) (tptr tvoid)])
+           (Scall None (Evar _free (Tfunction (Ctypes.Tcons (tptr tvoid) Ctypes.Tnil) tvoid cc_default))
+              [Etempvar _l__2 (tptr (Tstruct _lock_t noattr))]))))
+  (normal_ret_assert
+     (PROP (0 <= i + 1 <= 6; Forall isptr flocks; Forall isptr glocks)
+      LOCAL (temp _i__2 (vint i); temp _t'1 p; lvar _thread_locks (tarray (tptr (Tstruct _lock_t noattr)) 6) lvar0;
+      gvar _q0 q0)
+      SEP (ghost_factory; data_at (fst (Znth 0 gshs2 (gsh', gsh'))) (tptr tqueue_t) p q0;
+      fold_right sepcon emp
+        (firstn (Z.to_nat (i + 1))
+           (map (fun sh : Share.t => data_at sh (tptr tqueue_t) p q0) (map snd (rev gshs1 ++ rev gshs2))));
+      lqueue (fst (Znth 0 lshs2 (lsh', lsh'))) gsh2 p ghosts lock;
+      fold_right sepcon emp
+        (firstn (Z.to_nat (i + 1))
+           (map (fun sh : Share.t => lqueue sh gsh2 p ghosts lock) (map snd (rev lshs1 ++ rev lshs2))));
+      EX ns : list Z,
+      !! (Zlength ns = Zlength ghosts) &&
+      fold_right sepcon emp
+        (firstn (Z.to_nat (i + 1) - 3)
+           (map (fun x : Z * val => ghost gsh1 tint (vint (fst x)) (snd x)) (combine ns ghosts)));
+      fold_right sepcon emp (skipn (Z.to_nat (i + 1)) (map Interp (map f_lock (combine (upto 3) flocks))));
+      fold_right sepcon emp (skipn (Z.to_nat (i + 1) - 3) (map Interp (map g_lock (combine (upto 3) glocks))));
+      data_at Tsh (tarray (tptr (Tstruct _lock_t noattr)) 6) (flocks ++ glocks) lvar0))).
+Proof.
+  intros.
+  Intro ns; Intros.
+    forward.
+    { go_lower.
+      repeat apply andp_right; apply prop_right; auto.
+      apply Forall_Znth.
+      - rewrite Zlength_app; abstract omega.
+      - rewrite Forall_app; split; eapply Forall_impl; try eassumption; auto. }
+    destruct (Z_lt_dec i 3).
+    - rewrite app_Znth1; [|abstract omega].
+      forward_call (Znth i flocks Vundef, sh1, f_lock_pred (snd (Znth (2 - i) lshs1 (Tsh, Tsh)))
+        (snd (Znth (2 - i) gshs1 (Ews, Ews))) sh2 q0 p lock (Znth i flocks Vundef) ghosts gsh2).
+      { apply prop_right; rewrite eval_cast_neutral_is_pointer_or_null;
+          rewrite eval_cast_neutral_is_pointer_or_null; auto. }
+      { assert (length flocks = 3)%nat by (rewrite Zlength_correct in *; Omega0).
+        erewrite skipn_cons, !Znth_map', Znth_combine; auto;
+          [|rewrite !map_length, combine_length, Min.min_l; rewrite upto_length; Omega0].
+        rewrite Z2Nat.id; [|omega].
+        rewrite Znth_upto with (m := 3%nat); [|Omega0].
+        rewrite <- (Nat.add_1_r (Z.to_nat i)).
+        instantiate (1 := Vundef); simpl; cancel. }
+      freeze [2; 3; 4; 5; 6; 7; 8; 9; 10] FR.
+      forward_call (Znth i flocks Vundef, Tsh, Later (f_lock_pred (snd (Znth (2 - i) lshs1 (Tsh, Tsh)))
+        (snd (Znth (2 - i) gshs1 (Ews, Ews))) sh2 q0 p lock (Znth i flocks Vundef) ghosts gsh2)).
+      { apply prop_right; rewrite eval_cast_neutral_is_pointer_or_null;
+          rewrite eval_cast_neutral_is_pointer_or_null; auto. }
+      { simpl.
+        rewrite selflock_eq at 2.
+        rewrite (sepcon_comm (FRZL FR)); repeat rewrite sepcon_assoc.
+        eapply derives_trans; [apply sepcon_derives; [apply lock_inv_later | apply derives_refl]|].
+        rewrite <- (lock_inv_share_join sh1 sh2 Tsh); auto; cancel. }
+      { split; auto; split; [apply later_positive, f_inv_positive | apply later_rec, selflock_rec]. }
+      forward_call (Znth i flocks Vundef, sizeof tlock).
+      { rewrite data_at__memory_block; simpl; entailer!. }
+      Exists [0; 0; 0].
+      go_lower.
+      apply andp_right; [apply prop_right; repeat split; auto; abstract omega|].
+      apply andp_right; [apply prop_right; repeat split; auto|].
+      thaw FR.
+      rewrite Z2Nat.inj_add; try abstract omega; simpl.
+      assert (Z.to_nat i < 3)%nat by Omega0.
+      replace (Z.to_nat i + 1 - 3)%nat with O by abstract omega;
+        replace (Z.to_nat i - 3)%nat with O by abstract omega.
+      erewrite <- !firstn_app, <- !firstn_1_skipn.
+      rewrite !nth_Znth, !sepcon_app; simpl.
+      rewrite Z2Nat.id; try abstract omega.
+      rewrite !Znth_map', !app_Znth1; try (rewrite Zlength_rev; abstract omega).
+      rewrite !Znth_rev; try abstract omega.
+      rewrite Hglen1, Hlenl1.
+      replace (3 - i - 1) with (2 - i) by abstract omega.
+      unfold fold_right, lqueue; simpl; cancel.
+      entailer!.
+      apply derives_refl.
+      { rewrite !map_length, app_length, !rev_length.
+        rewrite Zlength_correct in *; Omega0. }
+      { rewrite !map_length, app_length, !rev_length.
+        rewrite Zlength_correct in *; Omega0. }
+    - rewrite app_Znth2; [|abstract omega].
+      replace (Zlength flocks) with 3 by auto.
+      assert (3 <= Z.to_nat i < 6)%nat.
+      { split; try Omega0.
+        rewrite Nat2Z.inj_le, Z2Nat.id; simpl; abstract omega. }
+      forward_call (Znth (i - 3) glocks Vundef, sh1, g_lock_pred (snd (Znth (2 - (i - 3)) lshs2 (lsh', lsh')))
+        (snd (Znth (2 - (i - 3)) gshs2 (gsh', gsh'))) sh2 q0 p lock (Znth (i - 3) glocks Vundef)
+        ghosts gsh1 gsh2 (Znth (i - 3) ghosts Vundef)).
+      { apply prop_right; rewrite eval_cast_neutral_is_pointer_or_null;
+          rewrite eval_cast_neutral_is_pointer_or_null; auto. }
+      { assert (length glocks = 3)%nat by (rewrite Zlength_correct in *; Omega0).
+        assert (3 > Z.to_nat i - 3)%nat by omega.
+        setoid_rewrite skipn_cons at 2;
+          [|rewrite !map_length, combine_length, Min.min_l; rewrite upto_length; auto; omega].
+        rewrite !Znth_map', Znth_combine, !Nat2Z.inj_sub, Z2Nat.id; auto; try omega.
+        rewrite Znth_upto with (m := 3%nat); [|simpl; omega].
+        rewrite <- (Nat.add_1_r (_ - _)).
+        instantiate (1 := Vundef); simpl; cancel. }
+      freeze [2; 3; 4; 5; 6; 7; 8; 9; 10] FR.
+      forward_call (Znth (i - 3) glocks Vundef, Tsh, Later (g_lock_pred
+        (snd (Znth (2 - (i - 3)) lshs2 (lsh', lsh')))
+        (snd (Znth (2 - (i - 3)) gshs2 (gsh', gsh'))) sh2 q0 p lock (Znth (i - 3) glocks Vundef)
+        ghosts gsh1 gsh2 (Znth (i - 3) ghosts Vundef))).
+      { apply prop_right; rewrite eval_cast_neutral_is_pointer_or_null;
+          rewrite eval_cast_neutral_is_pointer_or_null; auto. }
+      { simpl.
+        rewrite selflock_eq at 2.
+        rewrite (sepcon_comm (FRZL FR)); repeat rewrite sepcon_assoc.
+        eapply derives_trans; [apply sepcon_derives; [apply lock_inv_later | apply derives_refl]|].
+        rewrite <- (lock_inv_share_join sh1 sh2 Tsh); auto; cancel. }
+      { split; auto; split; [apply later_positive, g_inv_positive | apply later_rec, selflock_rec]. }
+      Intro x.
+      forward_call (Znth (i - 3) glocks Vundef, sizeof tlock).
+      { rewrite data_at__memory_block; simpl; entailer!. }
+      go_lower.
+      Exists (upd_Znth (i - 3) ns x).
+      apply andp_right; [apply prop_right; repeat split; auto; abstract omega|].
+      apply andp_right; [apply prop_right; repeat split; auto|].
+      thaw FR.
+      rewrite Z2Nat.inj_add; try abstract omega; simpl.
+      assert (Z.to_nat i < length gshs1 + length gshs2)%nat.
+      { rewrite Zlength_correct in *; Omega0. }
+      assert (Z.to_nat i < length lshs1 + length lshs2)%nat.
+      { rewrite Zlength_correct in *; Omega0. }
+      replace (Z.to_nat i + 1 - 3)%nat with (Z.to_nat i - 3 + 1)%nat by abstract omega.
+      assert (Zlength ns = 3).
+      { subst ghosts; rewrite !Zlength_cons, Zlength_nil in *; abstract omega. }
+      assert (length (upd_Znth (i - 3) ns x) = 3%nat).
+      { apply Nat2Z.inj.
+        rewrite <- Zlength_correct, upd_Znth_Zlength; simpl; abstract omega. }
+      erewrite <- !firstn_app, <- !firstn_1_skipn; try rewrite !map_length; try rewrite app_length, !rev_length;
+        try abstract omega.
+      rewrite !nth_Znth, !sepcon_app; simpl.
+      rewrite !Znth_map', !app_Znth2; try (rewrite Zlength_rev; abstract omega).
+      rewrite Nat2Z.inj_sub, Z2Nat.id; try abstract omega.
+      rewrite !Znth_rev; rewrite !Zlength_rev; try abstract omega.
+      rewrite interp_ghost, Znth_combine; auto; simpl.
+      instantiate (1 := Vundef); instantiate (1 := x).
+      rewrite upd_Znth_same; [|abstract omega].
+      assert (length flocks = 3%nat) by (rewrite Zlength_correct in *; Omega0).
+      rewrite skipn_short;
+        [|rewrite !map_length, combine_length, Min.min_l; rewrite upto_length; abstract omega].
+      setoid_rewrite skipn_short at 2;
+        [|rewrite !map_length, combine_length, Min.min_l; rewrite upto_length; abstract omega].
+      replace (Z.to_nat i - 3 + 1)%nat with (S (Z.to_nat i - 3))%nat by abstract omega.
+      rewrite Hglen1, Hlenl1, Hglen2, Hlenl2.
+      replace (3 - (i - 3) - 1) with (2 - (i - 3)) by abstract omega.
+      unfold fold_right, lqueue; simpl; cancel; entailer!.
+      + rewrite upd_Znth_Zlength; auto; abstract omega.
+      + rewrite sepcon_comm; apply sepcon_derives; [apply derives_refl|].
+        apply derives_refl'; f_equal.
+        replace (Z.to_nat i - 3)%nat with (Z.to_nat (i - 3)) by Omega0.
+        rewrite combine_upd_Znth1 with (d := Vundef), <- upd_Znth_map; try abstract omega.
+        rewrite <- !sublist_firstn, !sublist_upd_Znth_l; auto; try abstract omega.
+        rewrite Zlength_map.
+        rewrite Zlength_combine, Z.min_l; abstract omega.
+      + rewrite upd_Znth_Zlength; auto; abstract omega.
+      + rewrite combine_length, Min.min_r; subst ghosts; simpl; abstract omega.
+Qed.*)
+
+Lemma body_main:  semax_body Vprog Gprog f_main main_spec.
+Proof.
+  name q0 _q0; name locks _thread_locks; name results _results.
+  start_function.
+  destruct split_Ews as (gsh1 & gsh2 & ? & ? & Hgsh).
+  apply ghost_alloc.
+  apply new_ghost with (t := tint)(v := Vint (Int.repr (-1))); Intro g1.
+  apply new_ghost with (t := tint)(v := Vint (Int.repr (-1))); Intro g2.
+  apply new_ghost with (t := tint)(v := Vint (Int.repr (-1))); Intro g3.
+  set (ghosts := [g1; g2; g3]).
+  forward_call (gsh1, gsh2, ghosts).
+  { subst ghosts; simpl; cancel. }
+  Intro x; destruct x as (p, lock); simpl.
+  forward.
+  rewrite <- seq_assoc.
+  exploit (split_shares 3 Tsh); auto; intros (lshs1 & Hlenl1 & Hlshs1).
+  exploit (split_shares 3 Ews); auto; intros (gshs1 & Hglen1 & Hgshs1); simpl in *.
+  exploit (split_readable_share Tsh); auto; intros (sh1 & sh2 & ? & ? & Hsh).
+  set (f_lock := fun x => Lock_inv sh1 (snd x) (f_lock_pred (snd (Znth (2 - fst x) lshs1 (Tsh, Tsh)))
+    (snd (Znth (2 - fst x) gshs1 (Ews, Ews))) sh2 q0 p lock (snd x) ghosts gsh2)).
+  forward_for_simple_bound 3 (EX i : Z,
+    PROP ()
+    LOCAL (temp _t'1 p; lvar _thread_locks (tarray (tptr (Tstruct _lock_t noattr)) 6) lvar0; gvar _q0 q0)
+    SEP (ghost_factory; data_at (fst (Znth (3 - i) gshs1 (Ews, Ews))) (tptr tqueue_t) p q0;
+         lqueue (fst (Znth (3 - i) lshs1 (Tsh, Tsh))) gsh2 p ghosts lock;
+         ghost gsh1 tint (vint (-1)) g1; ghost gsh1 tint (vint (-1)) g2; ghost gsh1 tint (vint (-1)) g3;
+         EX flocks : list val, (!!(Zlength flocks = i) &&
+           (data_at Tsh (tarray (tptr (Tstruct _lock_t noattr)) 6) (flocks ++ repeat Vundef (Z.to_nat (6 - i))) lvar0 *
+            fold_right sepcon emp (map Interp (map f_lock (combine (upto (Z.to_nat i)) flocks))))))).
+  { go_lower; simpl.
+    Exists ([] : list val); entailer!.
+    do 2 (rewrite Znth_overflow; [|abstract omega]).
+    simpl; unfold data_at_, field_at_, data_at; entailer!. }
+  { apply main_loop1; auto. }
+  simpl; Intro flocks; Intros.
+  rewrite <- seq_assoc.
+  exploit (split_shares 3 (fst (Znth 0 lshs1 (Tsh, Tsh)))).
+  { exploit (Hlshs1 0); [abstract omega|].
+    destruct (Znth 0 lshs1 (Tsh, Tsh)); intros (? & ?); auto. }
+  intros (lshs2 & Hlenl2 & Hlshs2).
+  exploit (split_shares 3 (fst (Znth 0 gshs1 (Ews, Ews)))).
+  { exploit (Hgshs1 0); [abstract omega|].
+    destruct (Znth 0 gshs1 (Ews, Ews)) eqn: Hg; setoid_rewrite Hg; intros (? & ?); auto. }
+  intros (gshs2 & Hglen2 & Hgshs2); simpl in *.
+  set (lsh' := fst (Znth 0 lshs1 (Tsh, Tsh))).
+  set (gsh' := fst (Znth 0 gshs1 (Ews, Ews))).
+  set (g_lock := fun x => Lock_inv sh1 (snd x) (g_lock_pred
+    (snd (Znth (2 - fst x) lshs2 (lsh', lsh')))
+    (snd (Znth (2 - fst x) gshs2 (gsh', gsh')))
+    sh2 q0 p lock (snd x) ghosts gsh1 gsh2 (Znth (fst x) ghosts Vundef))).
+  forward_for_simple_bound 3 (EX i : Z,
+    PROP (Zlength flocks = 3)
+    LOCAL (temp _t'1 p; lvar _thread_locks (tarray (tptr (Tstruct _lock_t noattr)) 6) lvar0; gvar _q0 q0)
+    SEP (ghost_factory; data_at (fst (Znth (3 - i) gshs2 (gsh', gsh'))) (tptr tqueue_t) p q0;
+         lqueue (fst (Znth (3 - i) lshs2 (lsh', lsh'))) gsh2 p ghosts lock;
+         fold_right sepcon emp (skipn (Z.to_nat i) (map (ghost gsh1 tint (vint (-1))) ghosts));
+         fold_right sepcon emp (map Interp (map f_lock (combine (upto 3) flocks)));
+         EX glocks : list val, (!!(Zlength glocks = i) &&
+           (data_at Tsh (tarray (tptr (Tstruct _lock_t noattr)) 6) (flocks ++ glocks ++ repeat Vundef (Z.to_nat (3 - i))) lvar0 *
+            fold_right sepcon emp (map Interp (map g_lock (combine (upto (Z.to_nat i)) glocks))))))).
+  { go_lower; simpl.
+    Exists ([] : list val); entailer!.
+    do 2 (rewrite Znth_overflow with (i := 3); [simpl; cancel | abstract omega]). }
+  { apply main_loop2; auto. }
+  simpl; Intro glocks; Intros.
+  rewrite <- seq_assoc.
+  forward_for_simple_bound 6 (EX i : Z,
+    PROP (Forall isptr flocks; Forall isptr glocks)
+    LOCAL (temp _t'1 p; lvar _thread_locks (tarray (tptr (Tstruct _lock_t noattr)) 6) lvar0; gvar _q0 q0)
+    SEP (ghost_factory; data_at (fst (Znth 0 gshs2 (gsh', gsh'))) (tptr tqueue_t) p q0;
+         fold_right sepcon emp (firstn (Z.to_nat i) (map (fun sh => data_at sh (tptr tqueue_t) p q0) (map snd (rev gshs1 ++ rev gshs2))));
+         lqueue (fst (Znth 0 lshs2 (lsh', lsh'))) gsh2 p ghosts lock;
+         fold_right sepcon emp (firstn (Z.to_nat i) (map (fun sh => lqueue sh gsh2 p ghosts lock) (map snd (rev lshs1 ++ rev lshs2))));
+         EX ns : list Z, (!!(Zlength ns = Zlength ghosts) &&
+           fold_right sepcon emp (firstn (Z.to_nat i - 3) (map (fun x => ghost gsh1 tint (vint (fst x)) (snd x)) (combine ns ghosts))));
+         fold_right sepcon emp (skipn (Z.to_nat i) (map Interp (map f_lock (combine (upto 3) flocks))));
+         fold_right sepcon emp (skipn (Z.to_nat i - 3) (map Interp (map g_lock (combine (upto 3) glocks))));
+         data_at Tsh (tarray (tptr (Tstruct _lock_t noattr)) 6) (flocks ++ glocks) lvar0)).
+  { go_lower; apply andp_right; [|rewrite app_nil_r; Exists [0; 0; 0]; entailer!].
+    Intros.
+    do 3 (destruct flocks; [Omega0|]).
+    do 3 (destruct glocks; [Omega0|]).
+    repeat rewrite Zlength_cons in *; unfold Z.succ in *.
+    assert (flocks = []) by (apply Zlength_nil_inv; abstract omega).
+    assert (glocks = []) by (apply Zlength_nil_inv; abstract omega).
+    Transparent upto.
+    subst; simpl.
+    rewrite (lock_inv_isptr _ v), (lock_inv_isptr _ v0), (lock_inv_isptr _ v1), (lock_inv_isptr _ v2),
+      (lock_inv_isptr _ v3), (lock_inv_isptr _ v4).
+    rewrite !sepcon_assoc, !sepcon_andp_prop', !sepcon_andp_prop.
+    repeat (apply derives_extract_prop; intro).
+    apply prop_right; repeat split; auto. }
+  { apply main_loop3; auto. }
+  Intro ns; Intros.
+  rewrite !Zfirstn_same; try (rewrite !Zlength_map, Zlength_app, !Zlength_rev; abstract omega).
+  rewrite !map_app, !sepcon_app, !map_rev, !sepcon_rev.
+  rewrite sepcon_comm; gather_SEP 1 2.
+  rewrite <- sepcon_assoc, data_at_shares_join; [|rewrite Hglen2; auto].
+  subst gsh'; rewrite data_at_shares_join; [|rewrite Hglen1; auto].
+  rewrite sepcon_comm; gather_SEP 2 3.
+  rewrite <- sepcon_assoc, lqueue_shares_join; [|rewrite Hlenl2; auto].
+  subst lsh'; rewrite lqueue_shares_join; [|rewrite Hlenl1; auto].
+  forward.
+  forward_call (gsh1, gsh2, p, ghosts, ns, lock).
+  { replace (Z.to_nat 6 - 3)%nat with (Z.to_nat 3)%nat by Omega0.
+    rewrite Zfirstn_same; simpl.
+    unfold fold_right at 3; cancel.
+    { rewrite Zlength_map, Zlength_combine, Z.min_l; try abstract omega.
+      subst ghosts; rewrite !Zlength_cons, Zlength_nil in *; abstract omega. } }
+  forward.
+  Exists lvar0; entailer!.
+Qed.
+
+Definition extlink := ext_link_prog prog.
+
+Definition Espec := add_funspecs (Concurrent_Espec unit _ extlink) extlink Gprog.
+Existing Instance Espec.
+
+(* Use semax_func_mono here. *)
+Lemma all_funcs_correct:
+  semax_func Vprog Gprog (prog_funct prog) Gprog.
+Proof.
+unfold Gprog, prog, prog_funct; simpl.
+repeat (apply semax_func_cons_ext_vacuous; [reflexivity | reflexivity |]).
+eapply semax_func_cons_ext; try reflexivity.
+{ intros; entailer!. }
+{ admit. }
+eapply semax_func_cons_ext; try reflexivity.
+{ admit. }
+{ admit. }
+semax_func_cons_ext.
+semax_func_cons_ext.
+semax_func_cons_ext.
+semax_func_cons_ext.
+semax_func_cons_ext.
+semax_func_cons_ext.
+semax_func_cons_ext.
+semax_func_cons_ext.
+semax_func_cons_ext.
+semax_func_cons_ext.
+semax_func_cons_ext.
+semax_func_cons body_get_request.
+semax_func_cons body_process_request.
+semax_func_cons body_q_new.
+semax_func_cons body_q_del.
+semax_func_cons body_q_add.
+semax_func_cons body_q_remove.
+semax_func_cons body_f.
+(* XX For some reason, precondition_closed can't prove that all the gvars
+   aren't local variables. *)
+apply semax_func_cons; 
+ [ reflexivity 
+ | repeat apply Forall_cons; try apply Forall_nil; auto; computable
+ | unfold var_sizes_ok; repeat constructor; simpl; computable | reflexivity
+ | | apply body_g | ].
+{ precondition_closed.
+  apply closed_wrtl_PROPx, closed_wrtl_LOCALx, closed_wrtl_SEPx.
+  repeat constructor; apply closed_wrtl_gvar; unfold is_a_local; simpl;
+    intros [? | ?]; try contradiction; discriminate. }
+(* Here it's just missing an auto. *)
+apply semax_func_cons; 
+ [ reflexivity 
+ | repeat apply Forall_cons; try apply Forall_nil; (*here*)auto; computable
+ | unfold var_sizes_ok; repeat constructor; simpl; computable | reflexivity
+ | precondition_closed | apply body_main | ].
+apply semax_func_nil.
+Admitted.
